chore(chap11): add Lemma 11.4 and 11.5.

ConcreteSemanticsChapter11/ConcreteSemantics11_Denotational.thy
@@ -40,4 +40,70 @@ proof -
     (*using \<open>lfp (W (bval b) (D c)) = W (bval b) (D c) (lfp (W (bval b) (D c)))\<close> by auto*)
 qed
 
+text\<open>Equivalence of denotational and big-step semantics:\<close>
+
+(*Lemma 11.4.*)
+lemma D_if_big_step:  "(c,s) \<Rightarrow> t \<Longrightarrow> (s,t) \<in> D(c)"
+proof(induction rule: big_step_induct)
+case (Skip s)
+  then show ?case 
+    by simp
+next
+  case (Assign x a s)
+  then show ?case 
+    by auto
+next
+  case (Seq c\<^sub>1 s\<^sub>1 s\<^sub>2 c\<^sub>2 s\<^sub>3)
+  then show ?case 
+    by auto
+next
+  case (IfTrue b s c\<^sub>1 t c\<^sub>2)
+  then show ?case 
+    by simp
+next
+  case (IfFalse b s c\<^sub>2 t c\<^sub>1)
+  then show ?case 
+    by simp
+next
+  case (WhileFalse b s c)
+  then show ?case 
+    using D_While_If by auto
+next
+  case (WhileTrue b s\<^sub>1 c s\<^sub>2 s\<^sub>3)
+  then show ?case 
+  proof -
+    have "(s\<^sub>1, s\<^sub>3) \<in> D (c;; WHILE b DO c)"
+      using D.simps(3) WhileTrue.IH(1) WhileTrue.IH(2) by blast
+    then show ?thesis
+      using D_While_If WhileTrue.hyps(1) by force
+  qed
+qed
+
+abbreviation Big_step :: "com \<Rightarrow> com_den" where
+"Big_step c \<equiv> {(s,t). (c,s) \<Rightarrow> t}"
+
+(*Lemma 11.5.*)
+lemma Big_step_if_D:  "(s,t) \<in> D(c) \<Longrightarrow> (s,t) \<in> Big_step c"
+proof(induction c arbitrary: s t)
+case SKIP
+  then show ?case 
+    by auto
+next
+  case (Assign x1 x2)
+  then show ?case by fastforce
+next
+  case (Seq c1 c2)
+  then show ?case by fastforce
+next
+  case (If x1 c1 c2)
+  then show ?case by (auto split: if_splits)
+next
+  case (While b c)
+  let ?B = "Big_step (WHILE b DO c)"
+  let ?f = "W (bval b) (D c)"
+  have "?f ?B \<subseteq> ?B" using While.IH by (auto simp: W_def)
+  then show ?case 
+    using D.simps(5) While.prems lfp_lowerbound by blast
+qed
+
 end
